RelationalSem.thy
@@ -17,22 +17,23 @@ natural:
  account_ongoing_calls old = account_ongoing_calls new \<Longrightarrow>
  account_state_natural_change old new"
 
-inductive world_turn :: "(account_state * instruction_result) \<Rightarrow> (account_state * variable_env) \<Rightarrow> bool"
+inductive world_turn :: "(account_state * program_result) \<Rightarrow> (account_state * variable_env) \<Rightarrow> bool"
 where
-  world_continue: "world_turn (orig, (InstructionContinue v)) (orig, v)"
-(* | world_call: commented out because we are not going into the deeper callee
+(*  world_continue: "world_turn (orig, (InstructionContinue v)) (orig, v)"*)
+(* TODO  enable this with invariant.
+| world_call:
   "account_state_natural_change old_state new_state \<Longrightarrow>
    build_venv_called old_state callargs next_venv \<Longrightarrow>
    \<not> (instruction_result_continuing old_result) \<Longrightarrow>
    world_turn (old_state, old_result) (next_state, next_venv)" *)
-| world_return:
+world_return:
   "account_state_natural_change account_state_going_out account_state_back \<Longrightarrow>
    build_venv_returned account_state_back result new_v \<Longrightarrow>
-   world_turn (account_state_going_out, (InstructionToWorld (_, _, _, _))) (account_state_back, new_v)"
+   world_turn (account_state_going_out, (ProgramToWorld (_, _, _, _))) (account_state_back, new_v)"
 | world_fail:
   "account_state_natural_change account_state_going_out account_state_back \<Longrightarrow>
    build_venv_failed account_state_back = Some new_v \<Longrightarrow>
-   world_turn (account_state_going_out, (InstructionToWorld (_, _, _, _))) (account_state_back, new_v)"
+   world_turn (account_state_going_out, (ProgramToWorld (_, _, _, _))) (account_state_back, new_v)"
 
 abbreviation next_instruction :: "variable_env \<Rightarrow> inst \<Rightarrow> bool"
 where
@@ -41,35 +42,29 @@ where
       i' # _ \<Rightarrow> i = i'
     | _ \<Rightarrow> False)"
 
-inductive contract_turn :: "(account_state * variable_env) \<Rightarrow> (account_state * instruction_result) \<Rightarrow> bool"
+inductive contract_turn :: "(account_state * variable_env) \<Rightarrow> (account_state * program_result) \<Rightarrow> bool"
 where
-  contract_to_continue:
+  contract_to_world:
   "build_cenv old_account = cenv \<Longrightarrow>
-   next_instruction old_venv i \<Longrightarrow>
-   instruction_sem old_venv cenv i = InstructionContinue continuing_v \<Longrightarrow>
-   contract_turn (old_account, old_venv) (old_account, InstructionContinue continuing_v)"
-| contract_to_world:
-  "build_cenv old_account = cenv \<Longrightarrow>
-   next_instruction old_venv i \<Longrightarrow>
-   instruction_sem old_venv cenv i = InstructionToWorld (act, opt_v, st, bal) \<Longrightarrow>
+   program_sem old_venv cenv (venv_prg_sfx old_venv) n = ProgramToWorld (act, opt_v, st, bal) \<Longrightarrow>
    account_state_going_out = update_account_state a act opt_v st bal \<Longrightarrow>
-   contract_turn (old_account, old_venv) (account_state_going_out, InstructionToWorld (act, opt_v, st, bal))"
+   contract_turn (old_account, old_venv) (account_state_going_out, ProgramToWorld (act, opt_v, st, bal))"
 | contract_annotation_failure:
   "build_cenv old_account = cenv \<Longrightarrow>
-   next_instruction old_venv i \<Longrightarrow>
-   instruction_sem old_venv cenv i = InstructionAnnotationFailure \<Longrightarrow>
-   contract_turn (old_account, old_venv) (old_account, InstrucitonAnnotationFailure)"
+   program_sem old_venv cenv (venv_prg_sfx old_venv) n = ProgramAnnotationFailure \<Longrightarrow>
+   contract_turn (old_account, old_venv) (old_account, ProgramAnnotationFailure)"
 
 
-inductive one_step :: "(account_state * instruction_result) \<Rightarrow> (account_state * instruction_result) \<Rightarrow> bool"
+inductive one_step :: "(account_state * program_result) \<Rightarrow> (account_state * program_result) \<Rightarrow> bool"
 where
 step:
 "world_turn a b \<Longrightarrow> contract_turn b c \<Longrightarrow> one_step a c"
 
-inductive initial_instruction_result :: "account_state \<Rightarrow> instruction_result \<Rightarrow> bool"
+inductive initial_program_result :: "account_state \<Rightarrow> (account_state * program_result) \<Rightarrow> bool"
 where
+initial:
 "bal (account_address a) = account_balance a \<Longrightarrow>
- initial_instruction_result a (InstructionToWorld (ContractFail, account_storage a, bal, None))"
+ initial_program_result a (a, ProgramToWorld (ContractFail, account_storage a, bal, None))"
 
 (* taken from the book Concrete Semantics *)
 inductive star :: "('a \<Rightarrow> 'a \<Rightarrow> bool) \<Rightarrow> 'a \<Rightarrow> 'a \<Rightarrow> bool"
@@ -77,47 +72,67 @@ where
 refl: "star r x x" |
 step: "r x y \<Longrightarrow> star r y z \<Longrightarrow> star r x z"
 
-inductive reachable :: "account_state \<Rightarrow> (account_state * instruction_result) \<Rightarrow> bool"
+(*
+inductive reachable :: "account_state \<Rightarrow> (account_state * program_result) \<Rightarrow> bool"
 where
-"initial_instruction_result original init \<Longrightarrow>
- star one_step (original, init) fin \<Longrightarrow>
+"star one_step init fin \<Longrightarrow>
+ initial_program_result original init \<Longrightarrow>
  reachable original fin"
+*)
 
-lemma star_ind :
+lemma star_case' :
 "
 star r init dst \<Longrightarrow>
-P init \<Longrightarrow>
+(P init) \<Longrightarrow>
 (\<forall> next future. r init next \<longrightarrow>
- star r next future \<longrightarrow> P future)
+ star r next future \<longrightarrow> (P future))
 \<Longrightarrow> P dst
 "
 apply(induction rule: star.induct; auto)
 done
 
-lemma reachable_ind :
-"(\<forall> init. initial_instruction_result a init \<longrightarrow>
-   (P (a, init) \<and>
-     (\<forall> next future. one_step (a, init) next \<longrightarrow>
-                     star one_step next future \<longrightarrow> P future )
-   )) \<Longrightarrow>
- reachable a f \<longrightarrow> P f"
-apply(rule impI)
-apply(erule reachable.cases)
+lemma star_case'' :
+"
+P init \<Longrightarrow>
+(\<forall> next future. r init next \<longrightarrow>
+ star r next future \<longrightarrow> P future) \<Longrightarrow>
+star r init dst \<longrightarrow> P dst
+"
 apply(auto)
-apply(erule star_ind; auto)
+apply(drule star_case'; auto)
 done
 
+lemma star_case :
+"star r a c \<Longrightarrow>
+ (a = c \<or> (\<exists> b. r a b \<and> star r b c))"
+apply(induction rule: star.induct; auto)
+done
+
+(*
+lemma reachable_ind :
+"\<forall> init. initial_program_result a init \<longrightarrow>
+    (P init \<and> (\<forall> next future. one_step init next \<longrightarrow> star one_step next future \<longrightarrow> P future)) \<Longrightarrow>
+ \<forall> fin. reachable a fin \<longrightarrow> P fin"
+apply(rule allI)
+apply(rule impI)
+apply(erule allE)
+apply(simp add: reachable.simps)
+apply(erule exE)
+*)
+
+(*
 inductive one_run :: "account_state \<Rightarrow> (account_state * instruction_result) \<Rightarrow> bool"
 where
 "initial_instruction_result original init \<Longrightarrow>
  one_step (original, init) fin \<Longrightarrow>
  one_run original fin"
-
+*)
 definition no_assertion_failure :: "account_state \<Rightarrow> bool"
 where
 "no_assertion_failure a ==
-  \<forall> fin. reachable a fin \<longrightarrow>
-  snd fin \<noteq> InstructionAnnotationFailure"
+  (\<forall> init. initial_program_result a init \<longrightarrow>
+  (\<forall> fin. star one_step init fin \<longrightarrow>
+  snd fin \<noteq> ProgramAnnotationFailure))"
 
 (* TODO: define calls_of_code *)
 
